# Chapter Exercises: Limits

## List of Exercises

### Exercise 1
Evaluate the following limit:
\[
\lim_{x \to 3} (2x + 1)
\]

---

### Exercise 2
Evaluate the following limit:
\[
\lim_{x \to -1} (x^2 + 2x + 3)
\]

---

### Exercise 3
Evaluate the following limit:
\[
\lim_{x \to 2} \frac{x^2 - 4}{x - 2}
\]

---

### Exercise 4
Evaluate the following limit:
\[
\lim_{x \to 0} \frac{5x}{x}
\]

---

### Exercise 5
Evaluate the following limit:
\[
\lim_{x \to 0^+} \frac{1}{x}
\]

---

### Exercise 6
Evaluate the following limit:
\[
\lim_{x \to 1} \frac{x^2 - 1}{x - 1}
\]

---

### Exercise 7
Evaluate the following limit:
\[
\lim_{x \to 2} \frac{x - 2}{x^2 - 4}
\]

---

### Exercise 8
Evaluate the following limit:
\[
\lim_{x \to 0} \frac{\sin(x)}{x}
\]

---

### Exercise 9
Evaluate the following limit:
\[
\lim_{x \to 0} \frac{1 - \cos(x)}{x}
\]

---

### Exercise 10
Evaluate the following limit:
\[
\lim_{x \to \infty} \frac{2x^2 + 3x + 1}{x^2 - x + 2}
\]

---

## Solutions

### Solution 1
For the limit:
\[
\lim_{x \to 3} (2x + 1)
\]
Substitute \(x = 3\) directly into the expression:
\[
2(3) + 1 = 7
\]
Thus, the limit is 7.

---

### Solution 2
For the limit:
\[
\lim_{x \to -1} (x^2 + 2x + 3)
\]
Substitute \(x = -1\):
\[
(-1)^2 + 2(-1) + 3 = 1 - 2 + 3 = 2
\]
Thus, the limit is 2.

---

### Solution 3
For the limit:
\[
\lim_{x \to 2} \frac{x^2 - 4}{x - 2}
\]
Factor the numerator:
\[
\frac{x^2 - 4}{x - 2} = \frac{(x - 2)(x + 2)}{x - 2}
\]
Cancel the common factor:
\[
= x + 2
\]
Now substitute \(x = 2\):
\[
2 + 2 = 4
\]
Thus, the limit is 4.

---

### Solution 4
For the limit:
\[
\lim_{x \to 0} \frac{5x}{x}
\]
For \(x \neq 0\), cancel the \(x\) terms:
\[
\frac{5x}{x} = 5
\]
Thus, the limit is 5.

---

### Solution 5
For the limit:
\[
\lim_{x \to 0^+} \frac{1}{x}
\]
As \(x \to 0^+\), \(\frac{1}{x}\) approaches \(+\infty\):
\[
\lim_{x \to 0^+} \frac{1}{x} = +\infty
\]
Thus, the limit is \(+\infty\).

---

### Solution 6
For the limit:
\[
\lim_{x \to 1} \frac{x^2 - 1}{x - 1}
\]
Factor the numerator:
\[
\frac{x^2 - 1}{x - 1} = \frac{(x - 1)(x + 1)}{x - 1}
\]
Cancel the common factor:
\[
= x + 1
\]
Now substitute \(x = 1\):
\[
1 + 1 = 2
\]
Thus, the limit is 2.

---

### Solution 7
For the limit:
\[
\lim_{x \to 2} \frac{x - 2}{x^2 - 4}
\]
Factor the denominator:
\[
\frac{x - 2}{(x - 2)(x + 2)} = \frac{1}{x + 2}
\]
Now substitute \(x = 2\):
\[
\frac{1}{2 + 2} = \frac{1}{4}
\]
Thus, the limit is \( \frac{1}{4} \).

---

### Solution 8
For the limit:
\[
\lim_{x \to 0} \frac{\sin(x)}{x}
\]
This is a standard limit result:
\[
\lim_{x \to 0} \frac{\sin(x)}{x} = 1
\]
Thus, the limit is 1.

---

### Solution 9
For the limit:
\[
\lim_{x \to 0} \frac{1 - \cos(x)}{x}
\]
Using the standard limit result:
\[
\lim_{x \to 0} \frac{1 - \cos(x)}{x} = 0
\]
Thus, the limit is 0.

---

### Solution 10
For the limit:
\[
\lim_{x \to \infty} \frac{2x^2 + 3x + 1}{x^2 - x + 2}
\]
For large \(x\), the highest degree terms dominate:
\[
\lim_{x \to \infty} \frac{2x^2}{x^2} = 2
\]
Thus, the limit is 2.

---

